Here is the analysis of the document, separated by page.

**Note:** The printed text in the document is in Sinhala and English/Mathematics. I have transcribed the Mathematical notation and English exactly. Where Sinhala text appears, I have indicated it as `[Sinhala text]` or translated the mathematical context where clear.

---

## Page 1

**Type:** Printed Exam Paper with Handwritten Solutions

### **Question 01**
**Printed Text:**
01. $f(x) = \sqrt{x^2 - 2x - 3}$ [Sinhala text asking for domain and range based on the graph]. $y = x^2 - 2x - 3$ [Sinhala text].

**Handwritten Solution:**
*   **Graph:** A hand-drawn parabola opening upwards.
    *   x-intercepts marked at $-1$ and $3$.
    *   Vertex minimum marked at coordinates $(1, -4)$ (implied by the $-4$ on y-axis).
    *   Shaded region on the x-axis for $x \leq -1$ and $x \geq 3$.
*   **Algebra:**
    $0 = x^2 - 2x - 3$
    $0 = (x-3)(x+1)$
    $x = 3 \quad x = -1$
*   **Result (Top Right):**
    $R_{f(x)} = [0, \infty)$ and $x \leq -1$ or $x \geq 3$

### **Question 02**
**Printed Text:**
02. $\frac{2}{x-1} \geq \frac{1}{x+2}$ [Sinhala text asking to find the range of x].

**Handwritten Solution:**
1.  $\frac{2}{x-1} - \frac{1}{x+2} \geq 0$
2.  $\frac{2(x+2) - (x-1)}{(x-1)(x+2)} \geq 0$
3.  $\frac{2x + 4 - x + 1}{(x-1)(x+2)} \geq 0$
4.  $\frac{x+5}{(x-1)(x+2)} \geq 0$
5.  Constraint: $x \neq 1, x \neq -2$
6.  **Visual:** A number line (sign chart) marked with critical points $-5, -2, 1$.
    *   Signs indicated: $(-)$ before -5, $(+)$ between -5 and -2, $(-)$ between -2 and 1, $(+)$ after 1.
7.  **Final Answer:** $x > 1$ or $-2 > x \geq -5$

---

## Page 2

**Type:** Printed Exam Paper with Handwritten Solutions

### **Question 03**
**Printed Text:**
03. ABCD [Sinhala text: Rhombus] $A=(1,3), B=(\frac{7}{3}, \frac{11}{3})$ [Sinhala text] $C=(3,5)$. D [Sinhala text: Find coordinates]. AC [Sinhala text] BD [Sinhala text: Find length and Area].

**Handwritten Solution:**
*   $AB = \sqrt{(1 - 7/3)^2 + (3 - 11/3)^2}$
*   Calculation simplifies to $AB = \frac{2\sqrt{5}}{3}$
*   Right side calculation: $AB = CD$
    $\frac{20}{9} = (3-x)^2 + (5-y)^2$
    $\frac{20}{9} = 9 - 6x + x^2 + 25 - 10y + y^2$
    $\frac{20}{9} = x^2 + y^2 - 6x - 10y + 34$

### **Question 04**
**Printed Text:**
04. $4\log_x 3 - 2\log_x x = 3^{\log_3 7}$ [Sinhala text: Solve equation].

**Handwritten Solution:**
*   $4\log_x 3 - 2\log_x x = 7$ (Simplifying $3^{\log_3 7}$ to 7)
*   $\frac{4}{\log_3 x} - 2(1) = 7$
*   $\frac{4}{\log_3 x} = 9$
*   $\log_3 x = \frac{4}{9}$
*   $x = 3^{4/9}$ (Implied, though not explicitly written in final line).

---

## Page 3

**Type:** Printed Exam Paper with Handwritten Solutions

### **Question 05**
**Printed Text:**
05. $\lim_{x \to 0} \frac{1 - \cos 6x + x \sin(5 \sin x)}{x^2}$ [Sinhala text: Find limit].

**Handwritten Solution:**
*   $\lim_{x \to 0}$ written, but no further steps shown.

### **Question 06**
**Printed Text:**
06. $P=(4a, 8a)$ [Sinhala text] $ay^2 = x^3$ [Sinhala text: Find equation of tangent and normal at P].

**Handwritten Solution:**
1.  $P \equiv (4a, 8a)$
2.  $a \cdot 2y \frac{dy}{dx} = 3x^2$
3.  $\frac{dy}{dx} = \frac{3x^2}{2ay}$
4.  At P: $\frac{3(4a)^2}{2a(8a)} = m$ (Gradient calculation)
5.  $m = \frac{3 \cdot 16a^2}{16a^2} = 3$
6.  Tangent equation: $y - 8a = 3(x - 4a)$
    $y - 8a = 3x - 12a$
    $3x - y - 4a = 0$
7.  Normal gradient: $m' = -1/3$ (implied by calculation below)
    $\frac{y - 8a}{x - 4a} = \frac{-1}{3}$ (Correction: Handwriting shows calculation for normal)
    $3(y - 8a) = -1(x - 4a)$
    $3y - 24a = -x + 4a$
    $x + 3y - 28a = 0$ (This line is cut off/messy but implied).
    *Actually written:* $3x^3 - 12x^2 a \dots$ (The bottom lines are messy algebra).

---

## Page 4

**Type:** Printed Exam Paper with Handwritten Solutions

### **Question 07**
**Printed Text:**
07. $k \in \mathbb{R}$ [Sinhala text] $f(x) = 2x^2 - 4kx + k + 1$. [Sinhala text: Find minimum value in terms of k. Find range of k for f(x) > 0 for all x].

**Handwritten Solution:**
1.  $f(x) = 2x^2 - 4kx + k + 1$
2.  $f'(x) = 4x - 4k$
3.  $f'(x) = 0 \Rightarrow x = k$
4.  Min value: $f(k) = 2k^2 - 4k(k) + k + 1 = -2k^2 + k + 1$
5.  For $f(x) > 0$ for all real x, Discriminant $\Delta < 0$ (or min value > 0).
    $-2k^2 + k + 1 > 0$
    $2k^2 - k - 1 < 0$
    $(2k + 1)(k - 1) < 0$
    Range: $-1/2 < k < 1$

### **Question 08**
**Printed Text:**
08. $x^3 = A(x-1)^3 + B(x-1)^2 + C(x-1) + D$ [Sinhala text: Find partial fractions].

**Handwritten Solution:**
1.  $x^3 = A(x^3 - 3x^2 + 3x - 1) + B(x^2 - 2x + 1) + C(x-1) + D$
2.  Comparing coefficients:
    *   $x^3$: $A = 1$
    *   $x^2$: $0 = -3A + B \Rightarrow B = 3$
    *   $x$: $0 = 3A - 2B + C \Rightarrow 0 = 3 - 6 + C \Rightarrow C = 3$
    *   Constant: $0 = -A + B - C + D \Rightarrow 0 = -1 + 3 - 3 + D \Rightarrow D = 1$
3.  Result: $x^3 = 1(x-1)^3 + 3(x-1)^2 + 3(x-1) + 1$
4.  Partial Fraction part: $\frac{x^3}{(x-1)^4} = \frac{A}{x-1} + \frac{B}{(x-1)^2} + \frac{C}{(x-1)^3} + \frac{D}{(x-1)^4}$
    Substituting values: $\frac{1}{x-1} + \frac{3}{(x-1)^2} + \frac{3}{(x-1)^3} + \frac{1}{(x-1)^4}$

---

## Page 5

**Type:** Printed Exam Paper (Mostly blank)

### **Question 09**
**Printed Text:**
09. $\cos \frac{\pi}{5} - \cos \frac{2\pi}{5} = \frac{1}{2}$ [Sinhala text: Show that].

**Handwritten Notes:**
*   $\cos \frac{\pi}{5} - \cos \frac{2\pi}{5}$
*   $2 \sin \frac{3\pi}{10} \sin \frac{\pi}{10}$ (Product to sum formula application attempt).

### **Question 10**
**Printed Text:**
10. $\frac{\sin 6A - \sin 2A}{2 \cos 4A + \cos 6A + \cos 2A} = \tan A$ [Sinhala text: Show that].
    [Sinhala text]: Hence show $\tan \frac{\pi}{12} = 2 - \sqrt{3}$.

---

## Page 6

**Type:** Printed Exam Paper (Part B)

**Printed Text:**
*   **11. (a)** Quadratic equations involving $\alpha, \beta$. Roots $\gamma \delta$ and $\delta \gamma$.
*   **11. (b)** Polynomial remainder theorem involving $f(x)$ and $g(x)$.
*   **12. (a)** $f(x) = 2x^2 + 6x + 1 + k(x^2+2)$. Find range of k.
*   **12. (b)** Polynomial division $f(x) = 5x^4 - 2x^3 + \dots$
*   **12. (c)** Reciprocal equation $x^4 - 5x^3 + 8x^2 - 5x + 1 = 0$. Use substitution $t = x + \frac{1}{x}$.
*   **13. (a)** Partial fractions for $\frac{2x}{(x+1)^2(x^2+1)}$.
*   **13. (b)** Graphs of $y = 3|x-2|$ and $y = 4x - x^2$. Solve inequality.
*   **13. (c)** Graph $y = |x+2| + |x-3| \leq 7$.
*   **14. (a)** Derivative of $\tan x$ from first principles.
*   **14. (b)** Differentiate: i) $\tan(2x^2-1)$, ii) $\tan^3(\tan^{-1} 2x)$, iii) $x^{\tan x}$.

---

## Page 7

**Type:** Printed Exam Paper (Part B continued)

**Printed Text:**
*   **14. (c)** Differential equations involving $y = (3+4x)e^{-2x}$ and parametric equations $x = \sin t, y = \sin at$.
*   **15. (a)** Curve sketching $f(x) = \frac{x^2(x+1)}{(x-1)^3}$. Show $f'(x) = \frac{-2x(2x+1)}{(x-1)^4}$. Find asymptotes, stationary points.
*   **15. (b)** Optimization: Cylinder surface area and cost minimization.
*   **16.** Trigonometry equations and Inverse Trigonometry.
*   **17.** Triangle properties (Sine/Cosine rules).

---

## Page 8

**Type:** Handwritten Solution (Start of detailed working)

**Content:** Solution to Question 14(a) - Derivative of $\tan x$ from first principles.

**Transcription:**
1.  $f(x) = \tan x$
2.  $\frac{dy}{dx} = \lim_{\delta x \to 0} \frac{f(x+\delta x) - f(x)}{\delta x}$
3.  $\frac{dy}{dx} = \lim_{\delta x \to 0} \frac{\tan(x+\delta x) - \tan x}{\delta x}$
4.  $\lim_{\delta x \to 0} \frac{\frac{\tan x + \tan \delta x}{1 - \tan x \tan \delta x} - \tan x}{\delta x}$
5.  $\lim_{\delta x \to 0} \frac{\tan x + \tan \delta x - \tan x - \tan^2 x \tan \delta x}{\delta x (1 - \tan x \tan \delta x)}$
6.  $\lim_{\delta x \to 0} \frac{\tan \delta x (1 + \tan^2 x)}{\delta x (1 - \tan x \tan \delta x)}$
7.  $\lim_{\delta x \to 0} \left( \frac{\tan \delta x}{\delta x} \right) \cdot \frac{\sec^2 x}{(1 - \tan x \tan \delta x)}$
8.  Since $\lim_{\delta x \to 0} \frac{\tan \delta x}{\delta x} = 1$ and $\tan \delta x \to 0$:
9.  $= 1 \cdot \frac{\sec^2 x}{1 - 0}$
10. $\frac{dy}{dx} = \sec^2 x$

---

## Page 9

**Type:** Handwritten Solution

**Content:** Solution to Question 14(b) and (c).

**Transcription:**
*   **14(b)(i):** $y = \tan(2x^2 - 1)$
    $\frac{dy}{dx} = \sec^2(2x^2 - 1) \times 4x$
*   **14(b)(ii):** $y = \tan^3(\tan^{-1} 2x)$
    $\frac{dy}{dx} = 3\tan^2(\tan^{-1} 2x) \times \sec^2(\tan^{-1} 2x) \times \frac{1}{1+(2x)^2} \times 2$
*   **14(b)(iii):** $y = x^{\tan x}$
    $\ln y = \tan x \ln x$
    $\frac{1}{y} \frac{dy}{dx} = \sec^2 x \ln x + \tan x \cdot \frac{1}{x}$
    $\frac{dy}{dx} = x^{\tan x} (\sec^2 x \ln x + \frac{\tan x}{x})$
*   **14(c):** $y = (3+4x)e^{-2x}$
    $\frac{dy}{dx} = 4e^{-2x} + (3+4x)(-2e^{-2x})$
    $\frac{dy}{dx} = e^{-2x} [4 - 6 - 8x] = e^{-2x}[-2 - 8x]$
    Second derivative calculation follows to prove the identity.

---

## Page 10

**Type:** Handwritten Solution

**Content:** Solution to Question 15(a) - Curve Sketching derivatives.

**Transcription:**
1.  $f(x) = \frac{x^2(x+1)}{(x-1)^3}$
2.  Differentiation using Quotient Rule:
    $f'(x) = \frac{(x-1)^3 [2x(x+1) + x^2] - x^2(x+1)[3(x-1)^2]}{(x-1)^6}$
3.  Simplification steps shown to reach:
    $f'(x) = \frac{-2x(2x+1)}{(x-1)^4}$
4.  Stationary points ($f'(x) = 0$):
    $-2x(2x+1) = 0$
    $x = 0$ or $x = -1/2$
5.  Coordinates:
    If $x = 0, y = 0$.
    If $x = -1/2, y = \frac{(-1/2)^2(1/2)}{(-3/2)^3} = \frac{1/8}{-27/8} = -1/27$.
6.  Asymptotes:
    Vertical: $x = 1$
    Horizontal: $y = 1$ (Limit as $x \to \infty$).

---

## Page 11

**Type:** Handwritten Solution

**Content:** Solution to Question 15(a) - Sign Table and Graph.

**Visual Elements:**
1.  **Sign Table:**
    *   Intervals: $x < -1/2$, $-1/2 < x < 0$, $0 < x < 1$, $1 < x$.
    *   $dy/dx$ signs: $(-), (+), (-), (-)$.
    *   Shape: Decreasing $\searrow$, Increasing $\nearrow$, Decreasing $\searrow$, Decreasing $\searrow$.
    *   Local Min at $(-1/2, -1/27)$. Local Max at $(0,0)$.
2.  **Graph:**
    *   Axes drawn.
    *   Vertical asymptote at $x=1$.
    *   Horizontal asymptote at $y=1$.
    *   Curve passes through origin $(0,0)$ (Max) and $(-1/2, -1/27)$ (Min).
    *   Curve approaches $y=1$ for large $x$.

---

## Page 12

**Type:** Handwritten Solution

**Content:** Solution to Question 15(b) - Optimization.

**Transcription:**
1.  **Constraints:** $0 < k < \infty$ (from previous part context).
2.  **Cylinder Problem:**
    *   Area $A = 2\pi r h + 2\pi r^2$ (Closed cylinder implied or similar).
    *   Volume $V = \pi r^2 h = 24\pi$
    *   $h = \frac{24}{r^2}$
3.  **Cost Function (implied):**
    *   $C = 2\pi r h (1) + 2\pi r^2 (3)$ (Cost weights 1 and 3).
    *   Substitute $h$: $C = 2\pi r (\frac{24}{r^2}) + 6\pi r^2$
    *   $C = \frac{48\pi}{r} + 6\pi r^2$
4.  **Differentiation:**
    *   $\frac{dC}{dr} = -\frac{48\pi}{r^2} + 12\pi r$
    *   Set $\frac{dC}{dr} = 0$ for min cost.
    *   $12\pi r = \frac{48\pi}{r^2}$
    *   $r^3 = 4$
    *   $r = \sqrt[3]{4}$
5.  **Find h:**
    *   $h = \frac{24}{r^2}$ calculation.

---

## Page 13

**Type:** Handwritten Solution

**Content:** Solution to Question 12(a) - Quadratic Range.

**Transcription:**
1.  $2x^2 + 6x + 1 + kx^2 + 2k = f(x)$
2.  $(2+k)x^2 + 6x + (2k+1) = f(x)$
3.  For range to be $\mathbb{R}$ or specific condition (unclear text), usually involves Discriminant $\Delta$.
4.  Case 1: $2+k > 0 \Rightarrow k > -2$.
5.  Discriminant $\Delta \leq 0$ (for function to be always positive/negative).
    $36 - 4(2k+1)(2+k) \leq 0$
    $9 - (2k^2 + 5k + 2) \leq 0$
    $2k^2 + 5k - 7 \geq 0$
    $(2k+7)(k-1) \geq 0$
    $k \geq 1$ or $k \leq -7/2$.
6.  Combined with $k > -2$, solution is $k \geq 1$.

---

## Page 14

**Type:** Handwritten Solution

**Content:** Solution to Question 12(b) - Polynomials.

**Transcription:**
1.  $f(x) = 5x^4 - 2x^3 + 3x^2 + 4x + 6$
2.  Divided by $(x+2)$, Remainder is 74 (Calculation: $f(-2) = 80 - (-16) + 12 - 8 + 6 = 106$? Calculation in image shows 74).
3.  Long Division setup shown:
    $\frac{5x^4 - 2x^3 + \dots}{x+2}$
4.  Quotient found: $5x^3 - 12x^2 + 27x - 50$ (approximate reading of messy handwriting).
5.  Identity: $5x^4 - \dots = (x+2)(Ax^3 + Bx^2 + Cx + D) + 74$.
6.  Comparing coefficients to find A, B, C, D.
    $A = 5$
    $2A + B = -2 \Rightarrow 10 + B = -2 \Rightarrow B = -12$.
    $2B + C = 3 \Rightarrow -24 + C = 3 \Rightarrow C = 27$.
    $2C + D = 4 \Rightarrow 54 + D = 4 \Rightarrow D = -50$.

---

## Page 15

**Type:** Handwritten Solution

**Content:** Continuation of Polynomials.

**Transcription:**
*   $5x^3 - 12x^2 + \dots$
*   Substitution of values into $g(x)$.
*   Reciprocal equation substitution $t = x + \frac{1}{x}$.

---

## Page 16

**Type:** Handwritten Solution

**Content:** Solution to Question 13(a) - Partial Fractions.

**Transcription:**
1.  $\frac{2x}{(x+1)^2(x^2+1)} = \frac{A}{x+1} + \frac{B}{(x+1)^2} + \frac{Cx+D}{x^2+1}$
2.  $2x = A(x+1)(x^2+1) + B(x^2+1) + (Cx+D)(x+1)^2$
3.  Coefficients comparison:
    *   $x^3$: $0 = A + C \Rightarrow C = -A$
    *   $x= -1$: $-2 = B(2) \Rightarrow B = -1$
    *   $x=0$: $0 = A + B + D \Rightarrow 0 = A - 1 + D$
4.  Solving system:
    $A = 0, C = 0, D = 1$.
5.  Final Answer: $\frac{-1}{(x+1)^2} + \frac{1}{x^2+1}$

---

## Page 17

**Type:** Handwritten Solution

**Content:** Solution to Question 13(b) - Modulus Graphs.

**Visual Elements:**
*   **Graph:**
    *   $y = 3|x-2|$: V-shape with vertex at $(2,0)$.
    *   $y = 4x - x^2$: Inverted parabola passing through $(0,0)$ and $(4,0)$. Vertex at $(2,4)$.
    *   Intersection points marked.
*   **Algebra:**
    *   Solve $3(x-2) = 4x - x^2$ for $x > 2$.
        $3x - 6 = 4x - x^2 \Rightarrow x^2 - x - 6 = 0 \Rightarrow (x-3)(x+2)=0$.
        $x=3$ (since $x>2$).
    *   Solve $-3(x-2) = 4x - x^2$ for $x < 2$.
        $-3x + 6 = 4x - x^2 \Rightarrow x^2 - 7x + 6 = 0 \Rightarrow (x-6)(x-1)=0$.
        $x=1$ (since $x<2$).
    *   Inequality solution: $1 < x < 3$.

---

## Page 18

**Type:** Handwritten Solution

**Content:** Solution to Question 13(c) - Modulus Graph.

**Visual Elements:**
*   **Graph:** $y = |x+2| + |x-3|$.
    *   Flat bottom "bucket" shape.
    *   Flat segment between $x=-2$ and $x=3$ at height $y=5$.
    *   Left arm slope -2, Right arm slope +2.
*   **Algebra:**
    *   Inequality: $|x+2| + |x-3| \leq 7$.
    *   Right side: $2x - 1 = 7 \Rightarrow 2x = 8 \Rightarrow x = 4$.
    *   Left side: $-2x + 1 = 7 \Rightarrow -2x = 6 \Rightarrow x = -3$.
    *   Solution: $-3 \leq x \leq 4$.

---

## Page 19

**Type:** Handwritten Solution

**Content:** Solution to Question 11(a) - Quadratic Proofs.

**Transcription:**
1.  $ax^2 + bx + c = 0$ roots $\alpha, \beta$.
    $\alpha + \beta = -b/a$, $\alpha\beta = c/a$.
2.  New roots $\gamma \delta$ and $\delta \gamma$ (Note: The notation is a bit unclear, likely $\gamma, \delta$ are roots of another equation or transformed).
3.  Derivation of equation with roots $\alpha^2, \beta^2$ or similar transformations.
    $x^2 - (\text{sum})x + (\text{product}) = 0$.

---

## Page 20

**Type:** Handwritten Solution

**Content:** Continuation of Question 11.

**Transcription:**
*   Transformations involving $y = x + 1/x$ or similar substitutions.
*   The handwriting is faint and messy, but involves substituting variables back into the quadratic form to find the required equation.
*   Final lines appear to check coefficients.